spCTLCa | move interpreter definitions into separate file

cpSTLC/cpSTLCa_Defs.v
@@ -1,11 +1,12 @@
 (* %%%%%%%%%%%%%%%%%%%%%%%%%%%%%%%%%%%%%%%%%%%%%%%%%%%%%%%%%%%%%%%%% *) 
 (* Simply Typed Lambda Calculus with simple Concept Parameters
    :: version a
+   Definitions
 
    Definitions of STLC are based on
    Sofware Foundations, v.4 
   
-   Last Update: Wed, 18 Jan 2017
+   Last Update: Thu, 19 Jan 2017
  %%%%%%%%%%%%%%%%%%%%%%%%%%%%%%%%%%%%%%%%%%%%%%%%%%%%%%%%%%%%%%%%%%% *) 
 
 
@@ -134,70 +135,6 @@ Inductive ty : Type :=
   | TConceptPrm : id -> ty -> ty   (* C # T *)
 .
 
-Fixpoint beq_ty (T1 T2 : ty) : bool :=
-  match T1, T2 with
-  | TBool, TBool => true
-  | TNat,  TNat  => true 
-  | TArrow T11 T12, TArrow T21 T22 =>
-      andb (beq_ty T11 T21) (beq_ty T12 T22)
-  | TConceptPrm C1 T1, TConceptPrm C2 T2 =>
-      andb (beq_id C1 C2) (beq_ty T1 T2)
-  | _, _ => false
-  end.
-
-Lemma beq_ty_refl : forall T1, beq_ty T1 T1 = true.
-Proof.
-  intros T1. induction T1; (simpl; auto).
-  - (* T1 -> T2 *)
-    rewrite -> IHT1_1. rewrite -> IHT1_2. reflexivity.
-  - (* C # T *)
-    rewrite -> IHT1. rewrite <- beq_id_refl. reflexivity.
-Qed.
-
-Lemma beq_ty__eq : forall T1 T2,
-    beq_ty T1 T2 = true -> T1 = T2.
-Proof.
-  intros T1. induction T1;
-  (intros T2; induction T2; intros H);
-    (* in some cases it's just reflexivity *)
-    try reflexivity;
-    (* in other cases we have impossible equalities as assumptions 
-       (such as TNat = TBool) *)
-    try solve_by_invert.
-  - (* T1_1 -> T1_2 = T2_1 -> T2_2 *)
-    simpl in H. apply andb_true_iff in H.
-    inversion H as [H1 H2].
-    apply IHT1_1 in H1. apply IHT1_2 in H2.
-    subst. reflexivity.
-  - (* C1 # T1 = C2 # T2 *)
-    simpl in H. apply andb_true_iff in H.
-    inversion H as [HC HT].
-    rewrite -> beq_id_true_iff in HC. subst.
-    apply IHT1 in HT. subst.
-    reflexivity.
-Qed.  
-
-Lemma beq_tyP : forall T1 T2, reflect (T1 = T2) (beq_ty T1 T2).
-Proof.
-  intros T1 T2. 
-  apply iff_reflect. split.
-  - (* T1 = T2 -> beq_ty T1 T2 = true *)
-    intros H. 
-    destruct T1; destruct T2;
-      (* in simple cases reflexivity *)
-      try reflexivity;
-      (* some cases give contra in assumption *)
-      try (inversion H).
-    + (* T2_1 -> T2_2 = T2_1 -> T2_2 *)
-      simpl. apply andb_true_iff. split.
-      apply beq_ty_refl. apply beq_ty_refl.
-    + (* C # T2 = C # T2 *)
-      rename i0 into C. simpl. apply andb_true_iff. split.
-      symmetry. apply beq_id_refl. apply beq_ty_refl. 
-  - (* beq_ty T1 T2 = true -> T1 = T2 *)
-    apply beq_ty__eq.
-Qed.
-
 (* ----------------------------------------------------------------- *)
 (** **** Terms *)
 
@@ -299,6 +236,7 @@ Inductive program : Type :=
 
 (** There are examples of concepts and programs in [cpSTLCa_Examples.v]. *)
 
+
 (* ################################################################# *)
 (** ** Typing *)
 
@@ -337,18 +275,6 @@ Inductive cty : Type := CTdef : id_ty_map -> cty.
 
 Definition find_ty := mids_find ty.
 Hint Unfold find_ty.
-
-Definition beq_cty (CT1 CT2 : cty) : bool :=
-  match CT1, CT2 with
-    CTdef c1, CTdef c2 => IdMap.equal beq_ty c1 c2            
-  end.
-
-(*Lemma beq_cty_refl : forall CT1, beq_cty CT1 CT1 = true.
-Proof.
-  intros CT1. induction CT1; simpl.
-  apply IdMap.equal_1.
-  unfold IdMap.Equivb. unfold IdMap.Equiv.
-Qed.*)
 
 (** Models are always defined for some concepts. Therefore, 
     a list of members and their types must be the same as in
@@ -410,12 +336,6 @@ Definition mstempty : mdlcontext := @empty mty.
 
 Definition concept_defined (st : cptcontext) (nm : id) : Prop := 
   st nm <> None.
-
-Definition concept_defined_b (st : cptcontext) (nm : id) : bool :=
-  match st nm with
-  | None   => false
-  | Some _ => true
-  end.
   
 Inductive type_valid (st : cptcontext) : ty -> Prop :=
   | type_valid_nat   : type_valid st TNat
@@ -432,21 +352,6 @@ Inductive type_valid (st : cptcontext) : ty -> Prop :=
 
 Hint Constructors type_valid. 
 
-(** We can also write a function [types_are_valid] to check that 
-    all types in a list are valid.
-*)
-
-Fixpoint type_valid_b (st : cptcontext) (t : ty) : bool :=
-  match t with
-  | TNat  => true
-  | TBool => true
-  | TArrow t1 t2     => andb (type_valid_b st t1)  (type_valid_b st t2)
-  | TConceptPrm c t1 => andb (concept_defined_b st c) (type_valid_b st t1)
-  end.
-
-Definition types_valid_b (st : cptcontext) (ts : list ty) : bool :=
-  List.forallb (fun t => type_valid_b st t) ts.
-
 (** Now we are ready to define a property "concept is well defined" *)
 
 Definition concept_welldefined (st : cptcontext) (C : conceptdef) : Prop :=
@@ -460,43 +365,6 @@ Definition concept_welldefined (st : cptcontext) (C : conceptdef) : Prop :=
   end.
 
 Hint Unfold concept_welldefined.
-
-(** There is a problem: it's quite cumbersome to check 
-    well-definedness of concept definitions in propositional style.
-    We could implement auxuliary tactics to make proofs easier,
-    but it's not very practical. 
-
-    It would be convenient to have an algorithm for 
-    checking name repetitions in a concept definition.
-    To check this, we need an effective set of ids. 
-    The one based on AVL trees is defined in [Maps.v].
-*)
-
-(** Let's write a function [ids_are_unique] to check name repetitions. *)
-
-Fixpoint ids_are_unique_recur (nmlist : list id) (nmset : id_set) : bool :=
-  match nmlist with
-  | [] => true
-  | nm :: nms => if ids_mem nm nmset 
-                 then false
-                 else  ids_are_unique_recur nms (ids_add nm nmset)
-  end.
-
-Definition ids_are_unique (names : list id) : bool :=
-  ids_are_unique_recur names ids_empty.
-
-(** And define a function to check that "concept is well defined" *)
-
-Definition concept_welldefined_b (st : cptcontext) (C : conceptdef) : bool :=
-  match C with
-    cpt_def cname cbody =>
-    let (fnames, ftypes) := split (map namedecl_to_pair cbody) in
-    andb
-      (** all names are distinct *)
-      (ids_are_unique fnames)
-      (** and all types are valid *)
-      (types_valid_b st ftypes)           
-  end.
 
 (** We have a symbol table for concepts, concept types, but
     we have not defined yet a relation on concept definitions and
@@ -513,17 +381,6 @@ Definition concept_has_type (cst : cptcontext) (C : conceptdef) (CT : cty) : Pro
   (** amount of concept members is the same as in the concept type *)
         /\ List.length cbody = IdMap.cardinal cnmtys
       end end.
-
-(** And we now need an algorithmical way to find type of a concept. *)
-
-Definition concept_type_check (cst : cptcontext) (C : conceptdef) : option cty :=
-  if concept_welldefined_b cst C 
-  then match C with cpt_def cname cbody =>
-      let cbody' := map namedecl_to_pair cbody in
-      Some (CTdef (map_from_list cbody'))
-  end
-  else 
-    None.
 
 (** At this point we cannot do more on contexts. To check models,
     we have to be able to typecheck terms (function definitions). 
@@ -753,107 +610,6 @@ where "CTable '$' MTable ';' Gamma '|-' t '\in' T"
 
 Hint Constructors has_type.
 
-(** And the corresponding typechecker. *)
-
-(** Looks for _term_ type of [x] in context [Gamma]. *)
-Definition context_get_type (Gamma : context) (x : id) : option ty :=
-  option_handle (Gamma x)
-                (fun (ctx_ty : ctxvarty) 
-                 => match ctx_ty with | tmtype T => Some T | _ => None end)
-                None.
-
-(** Looks for _concept_ type of [C] in context [Gamma]. *)
-Definition context_get_concept (CTable : cptcontext) 
-                               (Gamma : context) (c : id) : option cty :=
-  option_handle (Gamma c)
-                (fun (ctx_ty : ctxvarty) 
-                 => match ctx_ty with | cpttype C => CTable C | _ => None end)
-                None.
-
-(** The type checking function. *)
-Fixpoint type_check (CTable : cptcontext) (MTable : mdlcontext)
-         (Gamma : context) (t : tm) : option ty :=
-  let tycheck := type_check CTable MTable in
-  let process_nat_un := fun (t1 : tm) =>
-                          match tycheck Gamma t1 with
-                          | Some TNat => Some TNat
-                          | _ => None
-                          end in
-  let process_nat_bin := fun (t1 t2 : tm) =>
-                           match tycheck Gamma t1, tycheck Gamma t2 with
-                           | Some TNat, Some TNat => Some TNat
-                           | _, _ => None
-                           end in
-  let process_nat_bin_bool := fun (t1 t2 : tm) =>
-                           match tycheck Gamma t1, tycheck Gamma t2 with
-                           | Some TNat, Some TNat => Some TBool
-                           | _, _ => None
-                           end in
-  match t with
-  | tvar x => 
-      (* there must be x : T \in Gamma *)
-      context_get_type Gamma x
-  | tapp t1 t2 => 
-      (* if t1 : T11 -> T12, t2 : T11, then (t1 t2) : T12 *)
-      match tycheck Gamma t1, tycheck Gamma t2 with
-        | Some (TArrow T11 T12), Some T2 => 
-          if beq_ty T11 T2 then Some T12 else None
-        | _ , _=> None
-      end
-  | tabs x T11 t12 =>
-      (* if t12 : T12 in (Gamma, x:T11), then \x:T11.t12 : T11 -> T12  *)
-      match tycheck (update Gamma x (tmtype T11)) t12 with
-      | Some T12 => Some (TArrow T11 T12)
-      | _ => None
-      end
-  | tmapp t1 M =>
-      (* if t1 : C # T1 and M defines concept C, then (t1 # M) : T1 *)
-      match tycheck Gamma t1, MTable M with
-        | Some (TConceptPrm C T1), Some (MTdef C' Mbody) => 
-          if beq_id C C' then Some T1 else None
-        | _, _ => None
-      end
-  | tcabs c C t1 =>
-      (* if C is known concept, and t1 : T1 in (Gamma, c:C), then
-         \c#C.t1 : C # T1 *)
-      match CTable C, tycheck (update Gamma c (cpttype C)) t1 with
-        | Some CT, Some T1 => Some (TConceptPrm C T1)
-        | _, _ => None
-      end
-  | tcinvk c f =>
-      (* if c:C \in Gamma, C:CT \in CTable, and f:TF \in CT,
-         then c.f : TF *)
-      match context_get_concept CTable Gamma c with
-      | Some (CTdef Cbody) => find_ty f Cbody 
-      | None => None
-      end
-  | ttrue  => Some TBool
-  | tfalse => Some TBool
-  | tif t1 t2 t3 =>
-      let tycheck' := tycheck Gamma in
-      match tycheck' t1, tycheck' t2, tycheck' t3 with
-      | Some TBool, Some T, Some T' => if beq_ty T T' then Some T else None
-      | _, _, _ => None
-      end
-  | tnat n   => Some TNat
-  | tsucc t1 => process_nat_un t1
-  | tpred t1 => process_nat_un t1
-  | tplus  t1 t2 => process_nat_bin t1 t2
-  | tminus t1 t2 => process_nat_bin t1 t2
-  | tmult  t1 t2 => process_nat_bin t1 t2
-  | teqnat t1 t2 => process_nat_bin_bool t1 t2
-  | tlenat t1 t2 => process_nat_bin_bool t1 t2
-  | tlet x t1 t2 =>
-      (* if t1 : T1 and t2 : T2 \in (Gamma, x:T1), 
-         then (let x=t1 in t2) : T2 *)
-      match tycheck Gamma t1 with
-      | Some T1 => match tycheck (update Gamma x (tmtype T1)) t2 with
-                     | Some T2 => Some T2 | _ => None 
-                   end
-      | _ => None
-      end
-  end. 
-
 (* ----------------------------------------------------------------- *)
 (** **** Checking Model Definitions *)
 
@@ -865,12 +621,6 @@ Fixpoint type_check (CTable : cptcontext) (MTable : mdlcontext)
 
 Definition model_defined (st : mdlcontext) (nm : id) : Prop := 
   st nm <> None.
-
-Definition model_defined_b (st : mdlcontext) (nm : id) : bool :=
-  match st nm with
-  | None   => false
-  | Some _ => true
-  end.
 
 (** [model_member_valid] is a proposition stating that the given
     model member [nd] (name definition, [f := t]) is valid against
@@ -886,21 +636,6 @@ Definition model_member_valid (cst : cptcontext) (mst : mdlcontext)
     (** and [T] is a type of [t], that is [cst * mst ; empty |- t : T] *)
     /\ has_type cst mst ctxempty t T
   end.
-
-(** And [model_member_valid_b] is a corresponding function to
-    check member's validity. *)
-
-Definition model_member_valid_b (cst : cptcontext) (mst : mdlcontext)
-                                (fnmtys : id_ty_map) (nd : namedef) : bool :=
-  match nd with nm_def nm t =>
-    (** there is [nm : T] in a concept *)
-    match find_ty nm fnmtys with
-    (** and [T] is a type of [t], that is [cst * mst ; empty |- t : T] *)
-    | Some T => match type_check cst mst ctxempty t with
-                  | Some T' => if beq_ty T T' then true else false
-                  | _ => false  end
-    | _ => false
-  end end.
 
 (** Now we are ready to formally define what it means for a model
     to be well-defined. *)
@@ -928,32 +663,6 @@ Definition model_welldefined (cst : cptcontext) (mst : mdlcontext) (M : modeldef
 
 Hint Unfold model_welldefined.
 
-(** And we define a function to check that "model is well defined" *)
-
-Definition model_welldefined_b (cst : cptcontext) (mst : mdlcontext) 
-           (M : modeldef) : bool :=
-  match M with 
-    mdl_def mname C mbody =>
-    match (cst C) with
-    (** concept is defined in symbol table *)
-    | Some (CTdef fnmtys) =>
-      let (fnames, fterms) := split (map namedef_to_pair mbody) in
-    (** model members are the same as concept members *)
-      let fnmtys_list := mids_elements ty fnmtys in
-      let Cfnames := List.map fst fnmtys_list in
-      andb
-        (IdSet.equal (set_from_list fnames) (set_from_list Cfnames))
-      (andb
-    (** types of model member terms conincide with 
-        concept member types *)
-        (forallb (model_member_valid_b cst mst fnmtys) mbody)
-    (** amount of concept members is the same as model members
-        (together with previous condition it means that 
-        all concept members are defined correctly in a model) *)  
-        (beq_nat (IdMap.cardinal fnmtys) (List.length mbody)))
-    | _ => false     
-  end end.
-
 (** And we also need typing relation for models. *)
 
 Definition model_has_type (cst : cptcontext) (mst : mdlcontext) 
@@ -970,18 +679,6 @@ Definition model_has_type (cst : cptcontext) (mst : mdlcontext)
   (** amount of model members is the same as in the model type *)
         /\ List.length mbody = IdMap.cardinal mnmtms
       end end.
-
-(** And we now need an algorithmical way to find type of a model. *)
-
-Definition model_type_check (cst : cptcontext) (mst : mdlcontext) 
-           (M : modeldef) : option mty :=
-  if model_welldefined_b cst mst M
-  then match M with mdl_def mname C mbody =>
-       let mbody' := map namedef_to_pair mbody in
-       Some (MTdef C (map_from_list mbody'))
-  end
-  else 
-    None.
 
 (** _Note!_ No any evaluation is applied to model members (terms). 
     So model members have to be exactly reflected in the model type,
@@ -1013,21 +710,6 @@ Definition conceptsec_welldefined (cptsec : conceptsec) (cst : cptcontext) : Pro
                    /\ concept_has_type cst C CT)
          ) cptsec. 
 
-Definition conceptsec_welldefined_b (cptsec : conceptsec) : cptcontext * bool :=
-(* use fold_left to pass the right context along the check *)
-  fold_left 
-    (fun (acc : cptcontext * bool) (C : conceptdef) =>
-       let (cst, correct) := acc
-       in if correct then 
-            let ctp := concept_type_check cst C
-            in match ctp with
-                 | Some CT => (update cst (conceptdef__get_name C) CT, true)
-                 | None    => (cstempty, false)
-               end 
-          else (cstempty, false)
-    )
-    cptsec (cstempty, true).
-
 (** First, model section (list of model definitions) is also 
     to be well-formed. 
     That is there is a symbol table of models such that
@@ -1046,21 +728,6 @@ Definition modelsec_welldefined
                    /\ model_has_type cst mst M MT)
          ) mdlsec.
 
-Definition modelsec_welldefined_b (mdlsec : modelsec) (cst : cptcontext)
-           : mdlcontext * bool :=
-  fold_left 
-    (fun (acc : mdlcontext * bool) (M : modeldef) =>
-       let (mst, correct) := acc
-       in if correct then 
-            let mtp := model_type_check cst mst M
-            in match mtp with
-                 | Some MT => (update mst (modeldef__get_name M) MT, true)
-                 | None    => (mstempty, false)
-               end 
-          else (mstempty, false)
-    )
-    mdlsec (mstempty, true).
-
 (** And, finally, we can define what it means for the whole _program_
     to be well-typed (correct). *)
 
@@ -1073,21 +740,6 @@ Definition program_has_type (cst : cptcontext) (mst : mdlcontext)
     /\ modelsec_welldefined mdlsec cst mst
     (** Term is well typed *)
     /\ has_type cst mst ctxempty t T
-  end.
-
-Definition program_type_check (cst : cptcontext) (mst : mdlcontext)
-           (prg : program) : option ty :=
-  match prg with tprog cptsec mdlsec t =>
-    let (cst, cpt_good) := conceptsec_welldefined_b cptsec in
-    (** All concepts are well defined *)
-    if cpt_good then
-      let (mst, mdl_good) := modelsec_welldefined_b mdlsec cst in
-      (** All models are well defined *)
-      if mdl_good then
-        (** Term is well typed *)
-        type_check cst mst ctxempty t
-      else None
-    else None
   end.
 
 
