cpSTLC/cpSTLCa_Interpreter.v
@@ -1,0 +1,439 @@
+(* %%%%%%%%%%%%%%%%%%%%%%%%%%%%%%%%%%%%%%%%%%%%%%%%%%%%%%%%%%%%%%%%% *) 
+(* Simply Typed Lambda Calculus with simple Concept Parameters
+   :: version a
+   Interpreter
+
+   Definitions of STLC are based on
+   Sofware Foundations, v.4 
+  
+   Last Update: Thu, 19 Jan 2017
+ %%%%%%%%%%%%%%%%%%%%%%%%%%%%%%%%%%%%%%%%%%%%%%%%%%%%%%%%%%%%%%%%%%% *) 
+
+
+(* ***************************************************************** *)
+(** * cpSTLCa Static Analysis and Interpretation
+
+    (Simply Typed Lambda Calculus with simple Concept Parameters  
+     :: version a) *)
+(* ***************************************************************** *)
+(* ***************************************************************** *)
+
+Add LoadPath "../..".
+
+Require Import ConceptParams.BasicPLDefs.Maps.
+Require Import ConceptParams.BasicPLDefs.Relations.
+
+Require Import ConceptParams.BasicPLDefs.Utils.
+
+Require Import ConceptParams.AuxTactics.LibTactics.
+Require Import ConceptParams.AuxTactics.BasicTactics.
+
+Require Import ConceptParams.cpSTLC.cpSTLCa_Defs.
+
+Require Import Coq.Lists.List.
+Import ListNotations.
+Require Import Coq.Bool.Bool.
+
+Require Import Coq.omega.Omega.
+
+
+(* ################################################################# *)
+(** ** Syntax *)
+
+(* ----------------------------------------------------------------- *)
+(** **** Types *)
+
+Fixpoint beq_ty (T1 T2 : ty) : bool :=
+  match T1, T2 with
+  | TBool, TBool => true
+  | TNat,  TNat  => true 
+  | TArrow T11 T12, TArrow T21 T22 =>
+      andb (beq_ty T11 T21) (beq_ty T12 T22)
+  | TConceptPrm C1 T1, TConceptPrm C2 T2 =>
+      andb (beq_id C1 C2) (beq_ty T1 T2)
+  | _, _ => false
+  end.
+
+
+(* ################################################################# *)
+(** ** Typing *)
+
+Definition beq_cty (CT1 CT2 : cty) : bool :=
+  match CT1, CT2 with
+    CTdef c1, CTdef c2 => IdMap.equal beq_ty c1 c2            
+  end.
+
+(*Lemma beq_cty_refl : forall CT1, beq_cty CT1 CT1 = true.
+Proof.
+  intros CT1. induction CT1; simpl.
+  apply IdMap.equal_1.
+  unfold IdMap.Equivb. unfold IdMap.Equiv.
+Qed.*)
+
+(* ================================================================= *)
+(** *** Checking Types Validity *)
+
+(* ----------------------------------------------------------------- *)
+(** **** Checking Concept Definitions *)
+
+Definition concept_defined_b (st : cptcontext) (nm : id) : bool :=
+  match st nm with
+  | None   => false
+  | Some _ => true
+  end.
+
+(** We can also write a function [types_are_valid] to check that 
+    all types in a list are valid.
+*)
+
+Fixpoint type_valid_b (st : cptcontext) (t : ty) : bool :=
+  match t with
+  | TNat  => true
+  | TBool => true
+  | TArrow t1 t2     => andb (type_valid_b st t1)  (type_valid_b st t2)
+  | TConceptPrm c t1 => andb (concept_defined_b st c) (type_valid_b st t1)
+  end.
+
+Definition types_valid_b (st : cptcontext) (ts : list ty) : bool :=
+  List.forallb (fun t => type_valid_b st t) ts.
+
+(** There is a problem: it's quite cumbersome to check 
+    well-definedness of concept definitions in propositional style.
+    We could implement auxuliary tactics to make proofs easier,
+    but it's not very practical. 
+
+    It would be convenient to have an algorithm for 
+    checking name repetitions in a concept definition.
+    To check this, we need an effective set of ids. 
+    The one based on AVL trees is defined in [Maps.v].
+*)
+
+(** Let's write a function [ids_are_unique] to check name repetitions. *)
+
+Fixpoint ids_are_unique_recur (nmlist : list id) (nmset : id_set) : bool :=
+  match nmlist with
+  | [] => true
+  | nm :: nms => if ids_mem nm nmset 
+                 then false
+                 else  ids_are_unique_recur nms (ids_add nm nmset)
+  end.
+
+Definition ids_are_unique (names : list id) : bool :=
+  ids_are_unique_recur names ids_empty.
+
+(** And define a function to check that "concept is well defined" *)
+
+Definition concept_welldefined_b (st : cptcontext) (C : conceptdef) : bool :=
+  match C with
+    cpt_def cname cbody =>
+    let (fnames, ftypes) := split (map namedecl_to_pair cbody) in
+    andb
+      (** all names are distinct *)
+      (ids_are_unique fnames)
+      (** and all types are valid *)
+      (types_valid_b st ftypes)           
+  end.
+
+(** And we now need an algorithmical way to find type of a concept. *)
+
+Definition concept_type_check (cst : cptcontext) (C : conceptdef) : option cty :=
+  if concept_welldefined_b cst C 
+  then match C with cpt_def cname cbody =>
+      let cbody' := map namedecl_to_pair cbody in
+      Some (CTdef (map_from_list cbody'))
+  end
+  else 
+    None.
+
+(** At this point we cannot do more on contexts. To check models,
+    we have to be able to typecheck terms (function definitions). 
+    But terms may conist of model applications.
+ *)
+
+(* ================================================================= *)
+(** *** Typing of Terms *)
+
+(** Let's define a typechecker, which corresponds to 
+    [has_type] relation. *)
+
+(** Looks for _term_ type of [x] in context [Gamma]. *)
+Definition context_get_type (Gamma : context) (x : id) : option ty :=
+  option_handle (Gamma x)
+                (fun (ctx_ty : ctxvarty) 
+                 => match ctx_ty with | tmtype T => Some T | _ => None end)
+                None.
+
+(** Looks for _concept_ type of [C] in context [Gamma]. *)
+Definition context_get_concept (CTable : cptcontext) 
+                               (Gamma : context) (c : id) : option cty :=
+  option_handle (Gamma c)
+                (fun (ctx_ty : ctxvarty) 
+                 => match ctx_ty with | cpttype C => CTable C | _ => None end)
+                None.
+
+(** The type checking function. *)
+Fixpoint type_check (CTable : cptcontext) (MTable : mdlcontext)
+         (Gamma : context) (t : tm) : option ty :=
+  let tycheck := type_check CTable MTable in
+  let process_nat_un := fun (t1 : tm) =>
+                          match tycheck Gamma t1 with
+                          | Some TNat => Some TNat
+                          | _ => None
+                          end in
+  let process_nat_bin := fun (t1 t2 : tm) =>
+                           match tycheck Gamma t1, tycheck Gamma t2 with
+                           | Some TNat, Some TNat => Some TNat
+                           | _, _ => None
+                           end in
+  let process_nat_bin_bool := fun (t1 t2 : tm) =>
+                           match tycheck Gamma t1, tycheck Gamma t2 with
+                           | Some TNat, Some TNat => Some TBool
+                           | _, _ => None
+                           end in
+  match t with
+  | tvar x => 
+      (* there must be x : T \in Gamma *)
+      context_get_type Gamma x
+  | tapp t1 t2 => 
+      (* if t1 : T11 -> T12, t2 : T11, then (t1 t2) : T12 *)
+      match tycheck Gamma t1, tycheck Gamma t2 with
+        | Some (TArrow T11 T12), Some T2 => 
+          if beq_ty T11 T2 then Some T12 else None
+        | _ , _=> None
+      end
+  | tabs x T11 t12 =>
+      (* if t12 : T12 in (Gamma, x:T11), then \x:T11.t12 : T11 -> T12  *)
+      match tycheck (update Gamma x (tmtype T11)) t12 with
+      | Some T12 => Some (TArrow T11 T12)
+      | _ => None
+      end
+  | tmapp t1 M =>
+      (* if t1 : C # T1 and M defines concept C, then (t1 # M) : T1 *)
+      match tycheck Gamma t1, MTable M with
+        | Some (TConceptPrm C T1), Some (MTdef C' Mbody) => 
+          if beq_id C C' then Some T1 else None
+        | _, _ => None
+      end
+  | tcabs c C t1 =>
+      (* if C is known concept, and t1 : T1 in (Gamma, c:C), then
+         \c#C.t1 : C # T1 *)
+      match CTable C, tycheck (update Gamma c (cpttype C)) t1 with
+        | Some CT, Some T1 => Some (TConceptPrm C T1)
+        | _, _ => None
+      end
+  | tcinvk c f =>
+      (* if c:C \in Gamma, C:CT \in CTable, and f:TF \in CT,
+         then c.f : TF *)
+      match context_get_concept CTable Gamma c with
+      | Some (CTdef Cbody) => find_ty f Cbody 
+      | None => None
+      end
+  | ttrue  => Some TBool
+  | tfalse => Some TBool
+  | tif t1 t2 t3 =>
+      let tycheck' := tycheck Gamma in
+      match tycheck' t1, tycheck' t2, tycheck' t3 with
+      | Some TBool, Some T, Some T' => if beq_ty T T' then Some T else None
+      | _, _, _ => None
+      end
+  | tnat n   => Some TNat
+  | tsucc t1 => process_nat_un t1
+  | tpred t1 => process_nat_un t1
+  | tplus  t1 t2 => process_nat_bin t1 t2
+  | tminus t1 t2 => process_nat_bin t1 t2
+  | tmult  t1 t2 => process_nat_bin t1 t2
+  | teqnat t1 t2 => process_nat_bin_bool t1 t2
+  | tlenat t1 t2 => process_nat_bin_bool t1 t2
+  | tlet x t1 t2 =>
+      (* if t1 : T1 and t2 : T2 \in (Gamma, x:T1), 
+         then (let x=t1 in t2) : T2 *)
+      match tycheck Gamma t1 with
+      | Some T1 => match tycheck (update Gamma x (tmtype T1)) t2 with
+                     | Some T2 => Some T2 | _ => None 
+                   end
+      | _ => None
+      end
+  end. 
+
+(* ----------------------------------------------------------------- *)
+(** **** Checking Model Definitions *)
+
+(** Model definition is Ok if:
+    - concept name is defined;
+    - all concept members are defined in a model;
+    - model member types coincide with concept member types.
+*)
+
+Definition model_defined_b (st : mdlcontext) (nm : id) : bool :=
+  match st nm with
+  | None   => false
+  | Some _ => true
+  end.
+
+(** Function [model_member_valid_b] corresponds to the [model_member_valid]
+    relation of member's validity. *)
+
+Definition model_member_valid_b (cst : cptcontext) (mst : mdlcontext)
+                                (fnmtys : id_ty_map) (nd : namedef) : bool :=
+  match nd with nm_def nm t =>
+    (** there is [nm : T] in a concept *)
+    match find_ty nm fnmtys with
+    (** and [T] is a type of [t], that is [cst * mst ; empty |- t : T] *)
+    | Some T => match type_check cst mst ctxempty t with
+                  | Some T' => if beq_ty T T' then true else false
+                  | _ => false  end
+    | _ => false
+  end end.
+
+(** And we define a function to check that "model is well defined". *)
+
+Definition model_welldefined_b (cst : cptcontext) (mst : mdlcontext) 
+           (M : modeldef) : bool :=
+  match M with 
+    mdl_def mname C mbody =>
+    match (cst C) with
+    (** concept is defined in symbol table *)
+    | Some (CTdef fnmtys) =>
+      let (fnames, fterms) := split (map namedef_to_pair mbody) in
+    (** model members are the same as concept members *)
+      let fnmtys_list := mids_elements ty fnmtys in
+      let Cfnames := List.map fst fnmtys_list in
+      andb
+        (IdSet.equal (set_from_list fnames) (set_from_list Cfnames))
+      (andb
+    (** types of model member terms conincide with 
+        concept member types *)
+        (forallb (model_member_valid_b cst mst fnmtys) mbody)
+    (** amount of concept members is the same as model members
+        (together with previous condition it means that 
+        all concept members are defined correctly in a model) *)  
+        (beq_nat (IdMap.cardinal fnmtys) (List.length mbody)))
+    | _ => false     
+  end end.
+
+(** And we now need an algorithmical way to find type of a model. *)
+
+Definition model_type_check (cst : cptcontext) (mst : mdlcontext) 
+           (M : modeldef) : option mty :=
+  if model_welldefined_b cst mst M
+  then match M with mdl_def mname C mbody =>
+       let mbody' := map namedef_to_pair mbody in
+       Some (MTdef C (map_from_list mbody'))
+  end
+  else 
+    None.
+
+(* ----------------------------------------------------------------- *)
+(** **** Checking Programs *)
+
+Definition conceptsec_welldefined_b (cptsec : conceptsec) : cptcontext * bool :=
+(* use fold_left to pass the right context along the check *)
+  fold_left 
+    (fun (acc : cptcontext * bool) (C : conceptdef) =>
+       let (cst, correct) := acc
+       in if correct then 
+            let ctp := concept_type_check cst C
+            in match ctp with
+                 | Some CT => (update cst (conceptdef__get_name C) CT, true)
+                 | None    => (cstempty, false)
+               end 
+          else (cstempty, false)
+    )
+    cptsec (cstempty, true).
+
+Definition modelsec_welldefined_b (mdlsec : modelsec) (cst : cptcontext)
+           : mdlcontext * bool :=
+  fold_left 
+    (fun (acc : mdlcontext * bool) (M : modeldef) =>
+       let (mst, correct) := acc
+       in if correct then 
+            let mtp := model_type_check cst mst M
+            in match mtp with
+                 | Some MT => (update mst (modeldef__get_name M) MT, true)
+                 | None    => (mstempty, false)
+               end 
+          else (mstempty, false)
+    )
+    mdlsec (mstempty, true).
+
+Definition program_type_check (cst : cptcontext) (mst : mdlcontext)
+           (prg : program) : option ty :=
+  match prg with tprog cptsec mdlsec t =>
+    let (cst, cpt_good) := conceptsec_welldefined_b cptsec in
+    (** All concepts are well defined *)
+    if cpt_good then
+      let (mst, mdl_good) := modelsec_welldefined_b mdlsec cst in
+      (** All models are well defined *)
+      if mdl_good then
+        (** Term is well typed *)
+        type_check cst mst ctxempty t
+      else None
+    else None
+  end.
+
+
+(* ################################################################# *)
+(** ** Operational Semantics *)
+
+
+(* ================================================================= *)
+(** *** Substitution *)
+
+
+
+
+(*
+
+Fixpoint subst (x:id) (s:tm) (t:tm) : tm :=
+  match t with
+  | tvar y =>
+      if beq_id x y then s else t
+  | tabs y T t1 =>
+      tabs y T (if beq_id x y then t1 else (subst x s t1))
+  | tapp t1 t2 =>
+      tapp (subst x s t1) (subst x s t2)
+  | tnat n =>
+      tnat n
+  | tsucc t1 =>
+      tsucc (subst x s t1)
+  | tpred t1 =>
+      tpred (subst x s t1)
+  | tmult t1 t2 =>
+      tmult (subst x s t1) (subst x s t2)
+  | tif0 t1 t2 t3 =>
+      tif0 (subst x s t1) (subst x s t2) (subst x s t3)
+  | tpair t1 t2 =>
+      tpair (subst x s t1) (subst x s t2)
+  | tfst t1 =>
+      tfst (subst x s t1)
+  | tsnd t1 =>
+      tsnd (subst x s t1)
+  | tunit => tunit
+    (* [x := s] (let y = t1 in t2) *)           
+  | tlet y t1 t2 =>
+      tlet y (subst x s t1) (if beq_id x y then t2 else (subst x s t2))
+  | tinl T t1 =>
+      tinl T (subst x s t1)
+  | tinr T t1 =>
+      tinr T (subst x s t1)
+  | tcase t0 y1 t1 y2 t2 =>
+      tcase (subst x s t0)
+         y1 (if beq_id x y1 then t1 else (subst x s t1))
+         y2 (if beq_id x y2 then t2 else (subst x s t2))
+  | tnil T =>
+      tnil T
+  | tcons t1 t2 =>
+      tcons (subst x s t1) (subst x s t2)
+  | tlcase t1 t2 y1 y2 t3 =>
+      tlcase (subst x s t1) (subst x s t2) y1 y2
+        (if beq_id x y1 then
+           t3
+         else if beq_id x y2 then t3
+              else (subst x s t3))
+  | tfix t1 =>
+      tfix (subst x s t1)
+  end.
+
+Notation "'[' x ':=' s ']' t" := (subst x s t) (at level 20).
+
+ *)
