Makefile
@@ -102,6 +102,7 @@ VFILES:=BasicPLDefs/Maps.v\
   AuxTactics/LibTactics.v\
   AuxTactics/BasicTactics.v\
   cpSTLC/cpSTLCa_Defs.v\
+  cpSTLC/cpSTLCa_Interpreter.v\
   cpSTLC/cpSTLCa_Examples.v\
   cpSTLC/cpSTLCa_Props.v
 
